

[13.0017]

$$1) \quad P^{-1} = \frac{1}{2} \begin{pmatrix} 1 & 0 & -1 \\ 1 & -1 & 0 \\ 0 & 1 & 1 \end{pmatrix}$$

$$2) \quad P^{-1}AP = \begin{pmatrix} 8 & 0 & 0 \\ 0 & 6 & 0 \\ 0 & 0 & 4 \end{pmatrix} = D$$

donc $A = PDP^{-1}$

$$A^{27} = \underbrace{PDP^{-1}}_I \cdot \underbrace{PDP^{-1}}_I \cdot PDP^{-1} \dots PDP^{-1}$$

$$= P D^{27} P^{-1}$$

$$= \begin{pmatrix} 2^{26}(2^{27} + 3^{27}) & 2^{26}(4^{27} - 3^{27}) & 2^{53}(2^{27} - 1) \\ 2^{26}(2^{27} - 3^{27}) & 2^{26}(3^{27} + 4^{27}) & 2^{53}(2^{27} - 1) \\ 2^{26}(3^{27} - 2^{27}) & 2^{26}(4^{26} - 3^{26}) & 2^{53}(2^{27} + 1) \end{pmatrix}$$